\documentclass[12pt]{article}
 
\usepackage[margin=1in]{geometry} 
\usepackage{amsmath,amsthm,amssymb}
\usepackage{enumitem} 

\newcommand{\problem}[1]{
	\vskip 1em
	{\large \textbf{#1}}
}
 
\begin{document}

\title{CS 1511 Homework 19} % Replace X with the appropriate number
\author{Mathew Varughese, Justin Kramer, Zach Smith} 
\date{Wednesday, March 27}

\maketitle

\setlength{\parskip}{.2em}
\setlength\parindent{0pt}

\problem{35. a)}
The polynomial to replace z would be $\sum_{x=0}^{1}\prod_{y=0}^{1}\sum_{z=0}^{1} 1-(1-(xy(1-z))) * (1-((1-x)(1-y)z))$
After multiplication, this becomes $\sum_{x=0}^{1}\prod_{y=0}^{1}\sum_{z=0}^{1} 1-(1-(xy-xyz)) * (1 - (z(1 - y - x + xy)$

$1-(1-(xy-xyz)) * (1 - (z - zy - zx + zxy))$

$1 - ((1 - (z -zy - zx + zxy)) - (xy+xyz) + (xyz - xy^2z - x^2zy + zx^2y^2 - xyz^2 + xy^2z^2 + x^2yz^2 - x^2y^2z^2)$

$1 - (1 - z + zy + zx - zxy - xy - xyz + xyz - xy^2z - x^2zy + zx^2y^2 - xyz^2 + xy^2z^2 + x^2yz^2 - x^2y^2z^2$
\vskip 0.3cm
Which all finally becomes

$\sum_{x=0}^{1}\prod_{y=0}^{1}\sum_{z=0}^{1} 1 - (1 - z - yz + xz - xyz - xy - xy^2z - x^2zy + zx^2y^2 - xyz^2 + xy^2z^2 + x^2yz^2 - x^2y^2z^2)$

\problem{35. b)}
i. The integer S would start with the polynomial
$s(x) = \prod_{y=0}^{1}\sum_{z=0}^{1} 1 - (1 - z - yz + xz - xyz - xy - xy^2z - x^2zy + zx^2y^2 - xyz^2 + xy^2z^2 + x^2yz^2 - x^2y^2z^2)$
added together having 0 and 1 for x to get S. Here would be those steps.

\vskip 0.3cm
WORK NEEDED HERE

1. With x = 0, y = 0, z = 0

\vskip 0.3cm

ii. The polynomial is g(y) = $\sum_{z=0}^{1} 1 - (1 - z - yz + (1/3)z - (1/3)yz - (1/3)y - (1/3)y^2z - (1/3)^2zy + z(1/3)^2y^2 - (1/3)yz^2 + (1/3)y^2z^2 + (1/3)^2yz^2 - (1/3)^2y^2z^2)$

\vskip 0.3cm

iii. Arthur is checking if this second polynomial works such that g(0) * g(1) = s(1/3)
to see if there is any issue with s(1/3). If there is, then there is proof that
s(1/3) is inccorect.

\problem{35. c)}
i. The polynomial to replace z would now be 

$\sum_{x=0}^{1}\prod_{y=0}^{1}\sum_{z=0}^{1} 1 - (1 - z - yz + xz - xyz - xy - xyz - xzy + zxy - xyz + xyz + xyz - xyz)$

\vskip 0.3cm

ii. The integer S would be generated the same way as above,
with the polynomial $s(x) = \prod_{y=0}^{1}\sum_{z=0}^{1} 1 - (1 - z - yz + xz - xyz - xy - xyz - xzy + zxy - xyz + xyz + xyz - xyz)$

\vskip 0.3cm
WORK NEEDED HERE

1. With x = 0, y = 0, z = 1

\vskip 0.3cm
Here are the steps to find S:

\vskip 0.3cm

iii. The polynomial is g(y) =  $\sum_{z=0}^{1} 1 - (1 - z - yz + (1/3)z - (1/3)yz - (1/3)y - (1/3)yz - (1/3)zy + z(1/3)y - (1/3)yz + (1/3)yz + (1/3)yz - (1/3)yz)$

\vskip 0.3cm

iv.  Arthur is checking if this second polynomial works such that g(0) * g(1) = s(1/3)
to see if there is any issue with s(1/3). If there is, then there is proof that
s(1/3) is inccorect.
\end{document}